Fixed simulation relation

formal/inference/Inference.thy
@@ -312,53 +312,6 @@ lemma score_1: "score_1 e s = k_score 1 e s"
     done
   done
 
-inductive accepts_trace :: "transition_matrix \<Rightarrow> cfstate \<Rightarrow> registers \<Rightarrow> trace \<Rightarrow> bool" where
-  base: "accepts_trace e s d []" |
-  step: "\<exists>(s', T) |\<in>| possible_steps e s d l i.
-         apply_outputs (Outputs T) (join_ir i d) = (map Some p) \<and>
-         accepts_trace e s' (apply_updates (Updates T) (join_ir i d) d) t \<Longrightarrow>
-         accepts_trace e s d ((l, i, p)#t)"
-
-lemma accepts_trace_step:
-  "accepts_trace e s d ((l, i, p)#t) = (\<exists>(s', T) |\<in>| possible_steps e s d l i.
-         apply_outputs (Outputs T) (join_ir i d) = (map Some p) \<and>
-         accepts_trace e s' (apply_updates (Updates T) (join_ir i d) d) t)"
-  apply standard
-   defer
-   apply (simp add: accepts_trace.step)
-  apply (rule accepts_trace.cases)
-  by auto
-
-fun accepts_trace_prim :: "transition_matrix \<Rightarrow> cfstate \<Rightarrow> registers \<Rightarrow> trace \<Rightarrow> bool" where
-  "accepts_trace_prim _ _ _ [] = True" |
-  "accepts_trace_prim e s d ((l, i, p)#t) = (
-    let poss_steps = possible_steps e s d l i in
-    if fis_singleton poss_steps then
-      let (s', T) = fthe_elem poss_steps in
-      if apply_outputs (Outputs T) (join_ir i d) = (map Some p) then
-        accepts_trace_prim e s' (apply_updates (Updates T) (join_ir i d) d) t
-      else False
-    else
-      (\<exists>(s', T) |\<in>| poss_steps.
-         apply_outputs (Outputs T) (join_ir i d) = (map Some p) \<and>
-         accepts_trace_prim e s' (apply_updates (Updates T) (join_ir i d) d) t))"
-
-lemma accepts_trace_prim [code]: "accepts_trace e s d l = accepts_trace_prim e s d l"
-proof(induct l arbitrary: s d)
-case Nil
-  then show ?case
-    by (simp add: accepts_trace.base)
-next
-case (Cons a l)
-  then show ?case
-    apply (cases a)
-    apply (simp add: accepts_trace_step Let_def fis_singleton_alt)
-    by auto
-qed
-
-definition accepts_log :: "trace set \<Rightarrow> transition_matrix \<Rightarrow> bool" where
-  "accepts_log T e = (\<forall>t \<in> T. accepts_trace e 0 <> t)"
-
 definition directly_subsumes :: "iEFSM \<Rightarrow> iEFSM \<Rightarrow> cfstate \<Rightarrow> cfstate \<Rightarrow> transition \<Rightarrow> transition \<Rightarrow> bool" where
   "directly_subsumes e1 e2 s s' t1 t2 \<equiv> (\<forall>p. recognises_trace (tm e1) p \<and> gets_us_to s (tm e1) 0 <>  p \<longrightarrow>
                                              recognises_trace (tm e2) p \<and> gets_us_to s' (tm e2) 0 <>  p \<longrightarrow>
